backends/lean/Aeneas/Std/String.lean
@@ -5,6 +5,18 @@ namespace Aeneas.Std
 
 def Str := Slice U8
 
+/-- TODO: we shouldn't use `decide +native` but it seems we can't reduce it otherwise. -/
+def toStr (s : String) (h : s.toByteArray.size ≤ U32.max := by decide +native) : Str :=
+  ⟨ s.toByteArray.toList.map
+    (fun x => ⟨ x.toNat, by cases x; simp only [UInt8.toNat_ofBitVec, UScalarTy.U8_numBits_eq, Nat.reducePow]; omega  ⟩),
+    by
+      simp only [UScalarTy.U8_numBits_eq, Nat.reducePow, Fin.mk_uInt8ToNat, BitVec.ofFin_uInt8ToFin,
+        List.length_map]
+      -- TODO: there seems to be missing lemmas to relate `ByteArray.size` and `ByteArray.toList.size`
+      sorry ⟩
+
+example : Str := toStr "hello"
+
 @[rust_type "core::str::iter::Chars" (body := .opaque)]
 structure core.str.iter.Chars where
   iter : core.slice.iter.Iter U8
